Start elaborating on x64 semantics in F*

tools/Vale/test/Semantics.fst
@@ -1,24 +1,65 @@
 module Semantics
 
-type reg =
-  | EAX
-  | EBX
+open FStar.BaseTypes
+open FStar.UInt64
+(* REVIEW: Why can't I open this? 
+open FStar.Int.Cast *)
+open FStar.Map
+open FStar.Mul
 
-type opr =
-  | OReg  : r:reg -> opr
-  | OConst: n:int -> opr
+type reg =
+  | Rax
+  | Rbx
+  | Rcx
+  | Rdx
+  | Rsi
+  | Rdi
+  | Rbp
+  | Rsp
+  | R8
+  | R9
+  | R10
+  | R11
+  | R12
+  | R13
+  | R14
+  | R15
+
+type maddr =
+  | MConst : n:nat -> maddr
+  | MReg   : r:reg -> offset:int -> maddr
+  | MIndex : base:reg -> scale:int -> index:reg -> offset:int -> maddr
+
+(* REVIEW: Should const be int instead of uint64?  Int gives more flexibility, but 
+           it means that eval_operand has to return int, not uint64.
+           Same question for the regs field in state below *)
+type operand =
+  | OConst: n:uint64 -> operand
+  | OReg  : r:reg -> operand
+  | OMem  : m:maddr -> operand
+
+type dst_op = o:operand { not(OConst? o || (OReg? o && Rsp? (OReg?.r o) )) }
 
 type ocmp =
-  | OLe: o1:opr -> o2:opr -> ocmp
+  | OEq: o1:operand -> o2:operand -> ocmp
+  | ONe: o1:operand -> o2:operand -> ocmp
+  | OLe: o1:operand -> o2:operand -> ocmp
+  | OGe: o1:operand -> o2:operand -> ocmp
+  | OLt: o1:operand -> o2:operand -> ocmp
+  | OGt: o1:operand -> o2:operand -> ocmp
 
-type mem_opr =
-  | OMem: base:reg -> offset:int -> mem_opr
-  | OOpr: o:opr -> mem_opr
 
 type ins =
-  | InsImm : dstImm:reg -> imm:int -> ins
-  | InsIncr: dstIncr:mem_opr -> ins
-  | InsAdd : dstAdd:reg -> srdAdd:opr -> ins
+  | Mov64      : dst:dst_op -> src:operand -> ins
+  | Add64      : dst:dst_op -> src:operand -> ins
+  | AddLea64   : dst:dst_op -> src1:operand -> src2:operand -> ins
+  | AddCarry64 : dst:dst_op -> src:operand -> ins
+  | Sub64      : dst:dst_op -> src:operand -> ins
+  | Mul64      : src:operand -> ins
+  | IMul64     : dst:dst_op -> src:operand -> ins
+  | Xor64      : dst:dst_op -> src:operand -> ins
+  | Shr64      : dst:dst_op -> amt:operand -> ins
+  | Shl64      : dst:dst_op -> amt:operand -> ins
 
 (*
  * while construct has a loop invariant
@@ -28,23 +69,26 @@ type code =
   | Ins   : ins:ins -> code
   | Block : block:list code -> code
   | IfElse: ifCond:ocmp -> ifTrue:code -> ifFalse:code -> code
-  | While : whileCond:ocmp -> whileBody:code -> inv:mem_opr -> code
+  | While : whileCond:ocmp -> whileBody:code -> inv:operand -> code
 
 type codes = list code
 
 (* map type from the F* library, it needs the key type to have decidable equality, not an issue here *)
 type map (key:eqtype) (value:Type) = Map.t key value
 
+(* TODO: Eventually this should be a map to bytes.  Simplifying for now *)
+type mem = map int uint64
+
 (* state type, noeq qualifier means that this type does not have decidable equality (because of the maps) *)
 noeq type state = {
   ok  :bool;
-  regs:map reg int;
-  mem :map int int
+  regs:map reg uint64;
+  flags:uint64;
+  mem :mem;
 }
 
-assume val empty_reg:int
-
-open FStar.Map
+assume val invalid:uint64
+assume val havoc : state -> ins -> Tot uint64
 
 (* syntax for map accesses, m.[key] and m.[key] <- value *)
 let op_String_Access     = sel
@@ -53,56 +97,107 @@ let op_String_Assignment = upd
 (*
  * writing all the functions as Tot functions
  *)
- 
-let eval_reg (r:reg) (s:state) :int =
-  if s.regs `contains` r then s.regs.[r] else empty_reg
 
-let eval_mem (ptr:int) (s:state) :int =
-  if s.mem `contains` ptr then s.mem.[ptr] else empty_reg
+(* REVIEW: Is it preferred for r:reg to proceed s:state?  Does it come down to which one (if any) we're more likely to want to curry? *)
+let eval_reg (r:reg) (s:state) :uint64 =
+  if s.regs `contains` r then s.regs.[r] else invalid
 
-let update_reg (r:reg) (s:state) (i:int) :state = { s with regs = s.regs.[r] <- i }
+(*
+let valid_resolved_addr (ptr:int) (m:mem) :bool =
+  m `contains` ptr /\
+  m `contains` ptr + 1 /\
+  m `contains` ptr + 2 /\
+  m `contains` ptr + 3 
+*)
 
-let update_mem (ptr:int) (s:state) (i:int) :state = { s with mem = s.mem.[ptr] <- i }
+(* REVIEW: Is returning invalid the right thing to do here?  Seems like we want !state.ok if this happens *)
+let eval_mem (ptr:int) (s:state) :uint64 =
+  if s.mem `contains` ptr then s.mem.[ptr] else invalid
 
-let eval_opr (o:opr) (s:state) :int =
+let eval_maddr (m:maddr) (s:state) :int =
+  match m with
+  | MConst n -> n
+  | MReg reg offset -> (FStar.UInt64.v (eval_reg reg s)) + offset
+  | MIndex _ _ _ _ -> 42
+  (* TODO: Should be the following, but it doesn't type check for some reason
+  | MIndex base scale index offset -> (FStar.UInt64.v (eval_reg base s)) + (scale * (FStar.UInt64.v (eval_reg index s))) + offset
+  *)
+
+let eval_operand (o:operand) (s:state) :uint64 =
   match o with
-  | OReg r   -> eval_reg r s
   | OConst n -> n
+  | OReg r   -> eval_reg r s
+  | OMem m   -> eval_mem (eval_maddr m s) s
 
-let update_opr (o:opr) (s:state) (i:int) :state =
-  match o with
-  | OReg r   -> update_reg r s i
-   | OConst _ -> { s with ok = false }
-
-let eval_mem_opr (o:mem_opr) (s:state) :int =
-  match o with
-  | OMem base offset -> eval_mem ((eval_reg base s) + offset) s
-  | OOpr o           -> eval_opr o s
-
-let update_mem_opr (o:mem_opr) (s:state) (i:int) :state =
-  match o with
-  | OMem base offset -> update_mem ((eval_reg base s) + offset) s i
-  | OOpr o           -> update_opr o s i
-
-let mem_opr_ok (o:mem_opr) (s:state) :bool =
-  match o with
-  | OMem base offset -> s.mem `contains` ((eval_reg base s) + offset)
-  | OOpr _           -> true
-
+(* REVIEW: Is it strange to have a dangling v before each term? 
+   REVIEW: Do the boolean operators below mean what I think they mean? *)
 let eval_ocmp (s:state) (c:ocmp) :bool =
   match c with
-  | OLe o1 o2 -> (eval_opr o1 s) <= (eval_opr o2 s)
+  | OEq o1 o2 -> v (eval_operand o1 s) =  v (eval_operand o2 s)
+  | ONe o1 o2 -> v (eval_operand o1 s) <> v (eval_operand o2 s)
+  | OLe o1 o2 -> v (eval_operand o1 s) <= v (eval_operand o2 s)
+  | OGe o1 o2 -> v (eval_operand o1 s) >= v (eval_operand o2 s)
+  | OLt o1 o2 -> v (eval_operand o1 s) < v (eval_operand o2 s)
+  | OGt o1 o2 -> v (eval_operand o1 s) > v (eval_operand o2 s)
 
-let eval_ins_fn (ins:ins) (s:state) :state =
+let update_reg (r:reg) (s:state) (v:uint64) :state = { s with regs = s.regs.[r] <- v }
+
+let update_mem (ptr:int) (s:state) (v:uint64) :state = { s with mem = s.mem.[ptr] <- v }
+
+let update_operand (o:dst_op) (s:state) (v:uint64) :state =
+  match o with
+  | OReg r   -> update_reg r s v
+  | OMem m   -> update_mem (eval_maddr m s) s v
+
+let update_operand_and_flags (o:dst_op) (s:state) (ins:ins) (v:uint64) :state =
+  { (update_operand o s v) with flags = havoc s ins }
+
+(* REVIEW: Is there a cleaner way to write this? *)
+let cf (flags:uint64) :bool =
+  (v (logand flags (uint_to_t 1))) > 0
+
+(* REVIEW: Is there a way to write a numeric literal without a cast *)
+let update_cf (flags:uint64) (cf:bool) :uint64 =
+  if cf then logor flags (uint_to_t 1)
+  else flags
+
+(* REVIEW: How can I tell I got the constant on the next two lines correct? *)
+let uint32_max = 0x100000000
+let uint64_max = 0x10000000000000000
+
+(* REVIEW: What's the best way to handle "valid shift amount" for shift instructions?  It depends on ins and state *)
+let valid_shift_operand (o:operand) (s:state) :bool =
+  (OConst? o && 0 <= v (OConst?.n o) && v (OConst?.n o) < 32) 
+  || 
+  ((OReg? o) && (Rcx? (OReg?.r o)) && v (eval_operand o s) < uint32_max)
+
+let eval_ins (ins:ins) (s:state) :state =
   if not s.ok then s
   else
-    match ins with
-    | InsImm dstImm imm    -> update_reg dstImm s imm
-    | InsIncr dstIncr      ->
-      if mem_opr_ok dstIncr s
-      then update_mem_opr dstIncr s ((eval_mem_opr dstIncr s) + 1)
-      else { s with ok = false}
-    | InsAdd dstAdd srcAdd -> update_reg dstAdd s ((eval_reg dstAdd s) + (eval_opr srcAdd s))
+    match ins with 
+    | Mov64 dst src -> update_operand dst s (eval_operand src s)
+    | Add64 dst src -> update_operand_and_flags dst s ins (eval_operand dst s +%^ eval_operand src s)
+    | AddLea64 dst src1 src2 -> update_operand_and_flags dst s ins (eval_operand src1 s +%^ eval_operand src2 s)
+    | AddCarry64 dst src -> let old_carry = if cf(s.flags) then 1 else 0 in
+			   let sum = v (eval_operand dst s) + v (eval_operand src s) + old_carry in			  
+			   let new_carry = sum > uint64_max in
+			   { update_operand dst s (uint_to_t (sum % uint64_max)) with flags = update_cf s.flags new_carry }
+    | Sub64 dst src -> update_operand_and_flags dst s ins (eval_operand dst s -%^ eval_operand src s)
+    | Mul64 src -> let product = v (eval_reg Rax s) * v (eval_operand src s) in
+		  let hi = uint_to_t (product / uint64_max) in
+		  let lo = uint_to_t (product % uint64_max) in
+		  { update_reg Rax (update_reg Rdx s hi) lo with flags = havoc s ins }
+    | IMul64 dst src -> update_operand_and_flags dst s ins (eval_operand dst s *%^ eval_operand src s)	  
+    | Xor64 dst src -> update_operand_and_flags dst s ins (eval_operand dst s ^^ eval_operand src s)	  
+    | Shr64 dst amt -> if valid_shift_operand amt s then
+			 s
+			 (* REVIEW: Why doesn't the following work?
+			 update_operand_and_flags dst s ins (shift_right (eval_operand dst s) (UInt32.uint_to_t (v (eval_operand amt s)))) *)
+		        (* update_operand_and_flags dst s ins (shift_right (eval_operand dst s) (uint64_to_uint32 (eval_operand amt s))) *)	  
+		      else
+			{ s with ok = false }
+    | Shl64 dst amt -> s  (* TODO: Follow the format of Shr64, once it works *)
+
 
 (*
  * the decreases clause
@@ -110,7 +205,7 @@ let eval_ins_fn (ins:ins) (s:state) :state =
 let decr (c:code) (s:state) :nat =
   match c with
   | While _ _ inv ->
-    let n = eval_mem_opr inv s in
+    let n = v (eval_operand inv s) in
     if n >= 0 then n else 0
   | _             -> 0
 
@@ -119,27 +214,27 @@ let decr (c:code) (s:state) :nat =
  * None case arises when the while loop invariant fails to hold
  *)
 
-val eval_code_fn:  c:code           -> s:state -> Tot (option state) (decreases %[c; decr c s; 1])
-val eval_codes_fn: l:codes          -> s:state -> Tot (option state) (decreases %[l])
-val eval_while_fn: c:code{While? c} -> s:state -> Tot (option state) (decreases %[c; decr c s; 0])
+val eval_code:  c:code           -> s:state -> Tot (option state) (decreases %[c; decr c s; 1])
+val eval_codes: l:codes          -> s:state -> Tot (option state) (decreases %[l])
+val eval_while: c:code{While? c} -> s:state -> Tot (option state) (decreases %[c; decr c s; 0])
 
-let rec eval_code_fn c s =
+let rec eval_code c s =
   match c with
-  | Ins ins                       -> Some (eval_ins_fn ins s)
-  | Block l                       -> eval_codes_fn l s
-  | IfElse ifCond ifTrue ifFalse  -> if eval_ocmp s ifCond then eval_code_fn ifTrue s else eval_code_fn ifFalse s
-  | While _ _ _                   -> eval_while_fn c s
+  | Ins ins                       -> Some (eval_ins ins s)
+  | Block l                       -> eval_codes l s
+  | IfElse ifCond ifTrue ifFalse  -> if eval_ocmp s ifCond then eval_code ifTrue s else eval_code ifFalse s
+  | While _ _ _                   -> eval_while c s
     
-and eval_codes_fn l s =
+and eval_codes l s =
   match l with
   | []   -> Some s
   | c::tl ->
-    let s_opt = eval_code_fn c s in
-    if None? s_opt then None else eval_codes_fn tl (Some?.v s_opt)
+    let s_opt = eval_code c s in
+    if None? s_opt then None else eval_codes tl (Some?.v s_opt)
     
-and eval_while_fn c s_0 = (* trying to mimic the eval_while predicate using a function *)
+and eval_while c s_0 = (* trying to mimic the eval_while predicate using a function *)
   let While cond body inv = c in
-  let n_0 = eval_mem_opr inv s_0 in
+  let n_0 = v (eval_operand inv s_0) in
   let b = eval_ocmp s_0 cond in
 
   if n_0 <= 0 then
@@ -147,159 +242,12 @@ and eval_while_fn c s_0 = (* trying to mimic the eval_while predicate using a fu
   else  //loop invariant > 0
     if not b then None  //guard must evaluate to true
     else
-      let s_opt = eval_code_fn body s_0 in
+      let s_opt = eval_code body s_0 in
       if None? s_opt then None
       else
         let s_1 = Some?.v s_opt in
 	if not s_1.ok then Some s_1  //this is from the reference semantics, if ok flag is unset, return
 	else
-	  let n_1 = eval_mem_opr inv s_1 in
+	  let n_1 = v (eval_operand inv s_1) in
 	  if n_1 >= n_0 then None  //loop invariant must decrease
-	  else eval_while_fn c s_1
-
-(* now define the predicates as in the reference semantics *)
-let eval_ins (ins:ins) (s_0:state) (s_1:state) :Type0 = s_1 == eval_ins_fn ins s_0
-
-let eval_block (block:codes) (s_0:state) (sN:state) :Type0 =
-  eval_code_fn (Block block) s_0 == Some sN
-
-let eval_while (b:ocmp) (c:code) (inv:mem_opr) (s_0:state) (sN:state) :Type0 =
-  eval_while_fn (While b c inv) s_0 == Some sN
-
-let eval_code (c:code) (s_0:state) (sN:state) :Type0 =
-  eval_code_fn c s_0 == Some sN
-
-(***** Vale Interface *****)
-
-(*
- * what are the access qualifiers on the semantics above and interface below?
- *)
-
-type va_bool = bool
-type va_int = int
-type va_codes = codes
-type va_code = code
-
-type va_state = state
-let va_get_ok (s:va_state) :bool = s.ok
-let va_get_reg (r:reg) (s:va_state) :int = eval_reg r s
-let va_get_mem (s:va_state) :map int int = s.mem
-let va_update_ok (sM:va_state) (sK:va_state) :va_state  = { sK with ok = sM.ok }
-let va_update_reg (r:reg) (sM:va_state) (sK:va_state) :va_state = { sK with regs = sK.regs.[r] <- va_get_reg r sM }
-let va_update_mem (sM:va_state) (sK:va_state) :va_state = { sK with mem = sM.mem }
-
-
-type va_register = reg
-let va_op_register (r:reg) :va_register = r
-let va_is_src_register_int (r:reg) (s:va_state) :bool = true
-let va_is_dst_register (r:reg) (s:va_state) :bool = true
-let va_update_register (r:reg) (sM:va_state) (sK:va_state) :va_state = va_update_reg r sM sK
-let va_eval_register_int (s:va_state) (r:va_register) :int = eval_reg r s
-
-type va_operand = opr
-let va_op_operand_reg (r:reg) :va_operand = OReg r
-let va_is_src_operand_int (o:opr) (s:va_state) = true
-let va_is_dst_operand_int (o:opr) (s:va_state) = OReg? o
-let va_const_operand (o:opr{OReg? o}) (sM:va_state) (sK:va_state) :va_state = va_update_reg (OReg?.r o) sM sK
-let va_eval_operand_int (s:va_state) (o:va_operand) :int = eval_opr o s
-
-type va_mem_operand = mem_opr
-let va_op_mem_operand_reg (r:reg) :va_mem_operand = OOpr (OReg r)
-let va_op_mem_operand_operand (o:opr) :va_mem_operand = OOpr o
-let va_is_src_mem_operand_int (o:mem_opr) (s:va_state) :bool = mem_opr_ok o s
-let va_is_dst_mem_operand_int (o:mem_opr) (s:va_state) :bool = mem_opr_ok o s && (if OOpr? o then OReg? (OOpr?.o o) else true)
-let va_mem_const_operand (x:int) :va_mem_operand = OOpr (OConst x)
-let va_update_mem_operand (o:mem_opr{OOpr? o ==> OReg? (OOpr?.o o)}) (sM:va_state) (sK:va_state) :va_state =
-  match o with
-  | OMem base offset -> { sK with mem = sK.mem.[(eval_reg base sK) + offset] <- eval_mem_opr o sM }
-  | OOpr o           -> va_update_reg (OReg?.r o) sM sK
-let va_eval_mem_operand_int (s:va_state) (o:va_mem_operand) :int = eval_mem_opr o s
-
-type va_cmp = opr
-let va_op_cmp_reg (r:reg) :va_cmp = OReg r
-let va_const_cmp (x:int) :va_cmp = OConst x
-let va_eval_cmp_int (s:va_state) (r:va_cmp) :int = eval_opr r s
-
-let va_coerce_register_to_operand (r:va_register) :va_operand = OReg r
-
-let va_CNil () :va_codes = []
-let va_CCons (hd:va_code) (tl:va_codes) :va_codes = hd::tl
-let va_Block (block:va_codes) :va_code = Block block
-let va_IfElse (ifCond:ocmp) (ifTrue:va_code) (ifFalse:va_code) :va_code = IfElse ifCond ifTrue ifFalse
-let va_While (whileCond:ocmp) (whileBody:va_code) (inv:mem_opr) :va_code = While whileCond whileBody inv
-let va_cmp_le (a:va_operand) (b:va_operand) :ocmp = OLe a b
-let va_get_block (c:va_code{Block? c}) :va_codes = Block?.block c
-let va_get_ifCond (c:code{IfElse? c}) :ocmp = IfElse?.ifCond c
-let va_get_ifTrue (c:code{IfElse? c}) :code = IfElse?.ifTrue c
-let va_get_ifFalse (c:code{IfElse? c}) :code = IfElse?.ifFalse c
-let va_get_whileCond (c:code{While? c}) :ocmp = While?.whileCond c
-let va_get_whileBody (c:code{While? c}) :code = While?.whileBody c
-
-
-let va_state_eq (s_0:va_state) (s_1:va_state) :Type0 = s_0 == s_1
-
-let va_require (block:va_codes) (c:va_code) (s_0:va_state) (s_1:va_state) :Type0 =
-  Cons? block                         /\
-  Cons?.hd block == c                 /\
-  eval_code (va_Block block) s_0 s_1     /\
-  (forall (r:reg). s_0.regs `contains` r)  //what is this?
-
-let va_ensure (b_0:va_codes) (b_1:va_codes) (s_0:va_state) (s_1:va_state) (sN:va_state) :Type0 =
-  Cons? b_0                         /\
-  Cons?.tl b_0 == b_1                /\
-  eval_code (Cons?.hd b_0) s_0 s_1     /\
-  eval_code (va_Block b_1) s_1 sN     /\
-  (forall (r:reg). s_1.regs `contains` r)
-
-(* the lemmas have out variables, so writing them as pure functions *)
-
-(* abstract? *)
-
-let va_lemma_block (b_0:va_codes) (s_0:state) (sN:state)
-  :Pure (state * va_code * va_codes)
-        (requires (Cons? b_0 /\ eval_code (Block b_0) s_0 sN))
-        (ensures  (fun (s_1, c_1, b_1) -> b_0 == va_CCons c_1 b_1  /\
-	                           eval_code c_1 s_0 s_1 /\
-				   eval_code (va_Block b_1) s_1 sN))
-  = let c_1::b_1 = b_0 in
-    Some?.v (eval_code_fn c_1 s_0), c_1, b_1
-
-let va_lemma_empty (s_0:va_state) (sN:va_state)
-  :Pure va_state (requires (eval_code (Block (va_CNil ())) s_0 sN))
-                 (ensures  (fun sM -> sM == s_0 /\ sM == sN))
-  = s_0
-
-let va_lemma_ifElse (ifb:ocmp) (ct:code) (cf:code) (s_0:va_state) (sN:va_state)
-  :Pure (bool * va_state)
-        (requires (eval_code (IfElse ifb ct cf) s_0 sN))
-	(ensures  (fun (cond, sM) -> cond == eval_ocmp s_0 ifb /\
-	                          sM == s_0                 /\
-				  (if cond then eval_code ct sM sN else eval_code cf sM sN)))
-  = eval_ocmp s_0 ifb, s_0
-
-let va_whileInv (b:ocmp) (c:code) (inv:mem_opr) (s_0:va_state) (sN:va_state) =
-  eval_mem_opr inv s_0 >= 0           /\
-  (forall (r:reg). s_0.regs `contains` r) /\
-  eval_while b c inv s_0 sN
-
-let va_lemma_while (b:ocmp) (c:code) (inv:mem_opr) (s_0:va_state) (sN:va_state)
-  :Pure va_state
-        (requires (eval_code (While b c inv) s_0 sN))
-	(ensures  (fun s_1 -> eval_while b c inv s_0 sN /\ s_1 == s_0))
-  = s_0
-
-let va_lemma_whileTrue (b:ocmp) (c:code) (inv:mem_opr) (s_0:va_state) (sN:va_state)
-  :Pure (va_state * va_state)
-        (requires (eval_mem_opr inv s_0 > 0 /\
-	           eval_while b c inv s_0 sN))
-	(ensures  (fun (s_0', s_1) -> s_0' == s_0           /\
-	                          eval_ocmp s_0 b      /\
-				  eval_code c s_0' s_1 /\
-				  (if s_1.ok then eval_while b c inv s_1 sN else s_1 == sN)))
-  = s_0, Some?.v (eval_code_fn c s_0)
-
-let va_lemma_whileFalse (b:ocmp) (c:code) (inv:mem_opr) (s_0:va_state) (sN:va_state)
-  :Pure va_state (requires (eval_mem_opr inv s_0 == 0 /\
-                            eval_while b c inv s_0 sN))
-		 (ensures  (fun s_1 -> s_0 == s_1 /\ s_1 == sN /\ not (eval_ocmp s_0 b)))
-  = s_0
+	  else eval_while c s_1
